Added Abs_tstream2delayFun lemma. Renamed a few lemmata. Tried a few things.

TStream_DS.thy
@@ -25,76 +25,57 @@ oops
 lemma tsremdups_h_nbot [simp]: "ts\<noteq>\<bottom> \<Longrightarrow> tsRemDups_h\<cdot>ts\<cdot>None \<noteq> \<bottom>"
 oops
 
+(*
+lemma delayfun2tswell: "ts_well (\<up>\<surd> \<bullet> ts) \<Longrightarrow> ts_well ts"
+by (metis lscons_conv stream.sel_rews(5) ts_well_drop1 up_defined)
 
+lemma mlscons2tswell: "ts_well (\<up>(Msg m) \<bullet> ts) \<Longrightarrow> ts_well ts"
+by (metis lscons_conv stream.sel_rews(5) ts_well_drop1 up_defined)
+*)
  
-lift_definition tsExampIn :: "nat tstream" is "<[Msg 1, Msg 2, \<surd>, Msg 2, \<surd>]>"
+lift_definition tsExampInp :: "nat tstream" is "<[Msg 1, Msg 2, \<surd>, Msg 2, \<surd>]>"
 by (subst ts_well_def, auto)
 
-lift_definition tsExampResult :: "nat tstream" is "<[Msg 1, Msg 2, \<surd>,  \<surd>]>"  
+lift_definition tsExampOut :: "nat tstream" is "<[Msg 1, Msg 2, \<surd>,  \<surd>]>"  
 by (subst ts_well_def, auto)
 
-lemma "tsRemDups\<cdot>tsExampIn = tsExampResult"
-apply (simp add: tsExampIn_def tsExampResult_def tsremdups_insert)
-apply (subst absts2tsmlscons_msg2)
-apply (metis One_nat_def eq_onp_same_args list2s.simps(1) list2s.simps(2) lscons_conv sup'_def 
-       tsExampIn.rsp)
-apply (subst absts2tsmlscons_msg2)
-apply (metis sconc_scons ts_well_conc1 ts_well_sing_conc)
-by (smt Abs_tstream_strict Rep_Abs Rep_tstream_strict absts2delayfun absts2tsmlscons_msg2
-    discr.inject lscons_conv lscons_well n_not_Suc_n numeral_2_eq_2 sinftimes_unfold strictI
-    strict_icycle sup'_def tick_msg ts_well_conc tslscons_bot2 tslscons_nbot2 tsmlscons_lscons
-    tsremdups_h_delayfun tsremdups_h_mlscons tsremdups_h_strict tsremdups_h_tslscons_dup)
+lemma "tsRemDups\<cdot>tsExampInp = tsExampOut"
+apply (simp add: tsExampInp_def tsExampOut_def tsremdups_insert)
+using absts2tsmlscons2 absts2delayfun2 tsremdups_h_mlscons_dup tsremdups_h_mlscons_ndup
+      tsremdups_h_strict tsremdups_h_mlscons tsremdups_h_delayfun
+by (smt DiscrTick_def delayfun_nbot delayfun_tslscons_bot lscons_conv lscons_well msg_nwell
+    n_not_Suc_n numeral_2_eq_2 strictI sup'_def tick_msg ts_well_sing_conc tslscons_bot2)
+
+lift_definition tsExampInp2_1 :: "nat tstream" is "<[Msg 1, \<surd>, Msg 2, \<surd>]>"
+by (subst ts_well_def, auto)
+
+definition tsExampInp2_2 :: "bool stream" where 
+"tsExampInp2_2 = <[True, False]>"
+
+lift_definition tsExampOut2 :: "(nat \<times> bool) tstream" is "<[Msg (1, True), \<surd>, Msg (2, False), \<surd>]>"  
+by (subst ts_well_def, auto)
 
 lemma 
-  "tsZip\<cdot>(Abs_tstream (<[Msg 1, \<surd>, Msg 2, \<surd>]>))\<cdot>(<[True, False]>) = Abs_tstream (<[Msg (1, True), \<surd>, Msg (2, False), \<surd>]>)"
+  "tsZip\<cdot>tsExampInp2_1\<cdot>tsExampInp2_2 = tsExampOut2"
+apply (simp add: tsExampInp2_1_def tsExampInp2_2_def tsExampOut2_def)
+using absts2tsmlscons2 absts2delayfun2 tszip_mlscons tszip_delayfun tszip_mlscons_2msg 
+      tszip_mlscons_msgdelayfun tszip_mlscons_2msg_bot tszip_strict
 proof -
-  have f1: "updis (\<surd>::'a event) && <[]> = \<up>\<surd>"
-    by (simp add: sup'_def)
-  then have f2: "ts_well (updis (\<surd>::'a event) && <[]>)"
-    by (metis tick_msg)
-  have f3: "ts_well (updis (\<M> 2::'a) && <[\<surd>]>)"
-    by auto
-  have f4: "delayFun\<cdot>(Abs_tstream (updis (\<M> 2::'a) && <[\<surd>]>)) = Abs_tstream (updis \<surd> && <[]>) \<bullet> Abs_tstream (updis (\<M> 2) && <[\<surd>]>)"
-    using f1 delayfun_insert by auto
-  have f5: "Rep_tstream (Abs_tstream (updis \<surd> && <[]>) \<bullet> Abs_tstream (updis (\<M> 2::'a) && <[\<surd>]>)) = <[\<surd>, \<M> 2, \<surd>]>"
-    using f3 f2 f1 by (metis (no_types) list2s.simps(2) lscons_conv tsconc_rep_eq1)
-  have f6: "updis (\<surd>::('a \<times> bool) event) && <[]> = \<up>\<surd>"
-    by (metis list2s_0 sup'_def)
-  have f7: "Rep_tstream (Abs_tstream (updis (\<surd>::('a \<times> bool) event) && <[]>) \<bullet> \<bottom>) = <[\<surd>]>"
-    by (simp add: lscons_conv)
-  have f8: "tsMLscons\<cdot>(updis (2::'a))\<cdot>(delayFun\<cdot>\<bottom>) = Abs_tstream (updis (\<M> 2) && <[\<surd>]>)"
-    by (simp add: delayfun_insert tsmlscons_lscons3)
-  have f9: "Rep_tstream (Abs_tstream (updis \<surd> && <[]>) \<bullet> Abs_tstream (updis (\<M> (2::'a, False)) && <[\<surd>]>)) = (updis \<surd> && <[]>) \<bullet> updis (\<M> (2, False)) && <[\<surd>]>"
-    by (simp add: tsconc_rep_eq1)
-  have "Abs_tstream (updis \<surd> && <[]>) \<bullet> Abs_tstream (updis (\<M> (2::'a, False)) && <[\<surd>]>) \<noteq> \<bottom>"
-    using f6 by force
-  then have f10: "tsMLscons\<cdot>(updis (1::'a, True))\<cdot> (Abs_tstream (updis \<surd> && <[]>) \<bullet> Abs_tstream (updis (\<M> (2, False)) && <[\<surd>]>)) = Abs_tstream (updis (\<M> (1, True)) && Rep_tstream (Abs_tstream (updis \<surd> && <[]>) \<bullet> Abs_tstream (updis (\<M> (2, False)) && <[\<surd>]>)))"
-    using tsmlscons_lscons3 by blast
-  have f11: "tsMLscons\<cdot>(updis (2::'a, False))\<cdot> (Abs_tstream (updis \<surd> && <[]>) \<bullet> \<bottom>) = Abs_tstream (updis (\<M> (2, False)) && Rep_tstream (Abs_tstream (updis \<surd> && <[]>) \<bullet> \<bottom>))"
-    by (simp add: lscons_conv tsmlscons_lscons3)
-  have "Abs_tstream (updis \<surd> && <[]>) \<bullet> Abs_tstream (updis (\<M> 2::'a) && <[\<surd>]>) \<noteq> \<bottom>"
-    using f1 by auto
-  then show ?thesis
-    using f11 f10 f9 f8 f7 f6 f5 f4 by (metis (no_types) delayfun_insert list2s.simps(2) list2s_0 lscons_conv tsmlscons_lscons3 tszip_mlscons_msgdelayfun tszip_strict(2))
+  have f1: "Abs_tstream (\<up>(\<M> Suc 0) \<bullet> \<up>\<surd> \<bullet> \<up>(\<M> 2) \<bullet> \<up>\<surd>) 
+             = tsMLscons\<cdot>(updis (Suc 0))\<cdot> (Abs_tstream (\<up>\<surd> \<bullet> \<up>(\<M> 2) \<bullet> \<up>\<surd>))"
+    by (metis (no_types) absts2tsmlscons2 sconc_scons ts_well_conc1 ts_well_sing_conc)
+  have f2: "updis True && updis False && \<epsilon> = \<up>True \<bullet> \<up>False"
+    by (metis lscons_conv sup'_def)
+  have f3: "tsZip\<cdot> (tsMLscons\<cdot>(updis (2::nat))\<cdot>(Abs_tstream (\<up>\<surd>)))\<cdot> (updis False && \<epsilon>) 
+              = Abs_tstream (\<up>(\<M> (2, False)) \<bullet> \<up>\<surd>)"
+    by (metis Abs_tstream_strict Rep_tstream_strict absts2delayfun absts2tsmlscons2 sup'_def
+        ts_well_Rep ts_well_sing_conc tszip_mlscons_msgdelayfun tszip_strict(1))
+  have "ts_well (\<up>(\<M> (Suc 0, True)) \<bullet> \<up>\<surd> \<bullet> \<up>(\<M> (2, False)) \<bullet> \<up>\<surd>)"
+    by (metis (no_types) sconc_scons ts_well_conc1 ts_well_sing_conc)
+  then show "tsZip\<cdot> (Abs_tstream (\<up>(\<M> Suc 0) \<bullet> \<up>\<surd> \<bullet> \<up>(\<M> 2) \<bullet> \<up>\<surd>))\<cdot> (\<up>True \<bullet> \<up>False) 
+               = Abs_tstream (\<up>(\<M> (Suc 0, True)) \<bullet> \<up>\<surd> \<bullet> \<up>(\<M> (2, False)) \<bullet> \<up>\<surd>)"
+    using f3 f2 f1 by (metis (no_types) absts2delayfun2 absts2tsmlscons2 ts_well_sing_conc 
+                       tszip_mlscons_msgdelayfun)
 qed
-
-(*
-definition tsZip_h :: "'a event stream \<rightarrow> 'b stream \<rightarrow> ('a \<times> 'b) event stream" where
-"tsZip_h \<equiv> fix\<cdot>(\<Lambda> h s q. if s = \<epsilon> \<or> q = \<epsilon> then \<epsilon> 
-                         else if shd s = \<surd> then \<up>\<surd> \<bullet> h\<cdot>(srt\<cdot>s)\<cdot>q
-                         else \<up>(\<M> (\<M>\<inverse> (shd s), shd q)) \<bullet> h\<cdot>(srt\<cdot>s)\<cdot>(srt\<cdot>q))"
-
-definition tsZip :: "'a tstream \<rightarrow> 'b stream \<rightarrow> ('a \<times> 'b) tstream" where
-"tsZip \<equiv> \<Lambda> ts s. Abs_tstream (tsZip_h\<cdot>(Rep_tstream ts)\<cdot>s)"
-
-definition tsRemDups_h :: "'a option event \<Rightarrow> 'a option event stream \<rightarrow> 'a option event stream" where
-"tsRemDups_h \<equiv> fix\<cdot>(\<Lambda> h. (\<lambda> q. (\<Lambda> s. if s = \<epsilon> then \<epsilon> 
-                                     else if shd s = \<surd> then (\<up>\<surd> \<bullet> h q\<cdot>(srt\<cdot>s))
-                                     else if shd s \<noteq> q then (\<up>(shd s) \<bullet> h (shd s)\<cdot>(srt\<cdot>s))
-                                     else h q\<cdot>(srt\<cdot>s))))"
-
-definition tsRemDups :: "'a tstream \<rightarrow> 'a tstream" where
-"tsRemDups \<equiv> \<Lambda> ts. Abs_tstream (smap (\<lambda>x. case x of Msg (Some m) \<Rightarrow> (Msg m))\<cdot>(tsRemDups_h (\<M> None)\<cdot>(Rep_tstream (tsMap Some\<cdot>ts))))"
-*)
 
 end  
